this has promise

Clean/Examples/Add32LawfulCircuit.lean
@@ -1,25 +1,29 @@
 import Clean.Utils.Primes
+import Clean.Circuit.ExplicitCircuit
 import Clean.Gadgets.Addition32.Addition32Full
 import Clean.Examples.AddOperations
 
 open Gadgets.Addition8FullCarry (add8_full_carry)
 open Gadgets.Addition32Full (add32_full Inputs)
 
--- `infer_lawful_circuit` / `infer_constant_lawful_circuits` seem to work for all circuits
-instance lawful : ConstantLawfulCircuits (add32_full (p:=p)) := by infer_constant_lawful_circuits
+-- `infer_explicit_circuit` seem to work for all circuits
+instance explicit : ConstantExplicitCircuits (add32_full (p:=p)) := by
+  apply ConstantExplicitCircuits.from_constant_length (by infer_explicit_circuit)
+  try intros
+  simp only [ExplicitCircuit.local_length]
+  ac_rfl
 
 @[reducible] def circuit32 input := add32_full (p:=p) input
-#eval LawfulCircuit.final_offset (circuit32 default) 0
-#eval LawfulCircuit.output (circuit32 default) 0
+#eval ExplicitCircuit.local_length (circuit32 default) 0
+#eval ExplicitCircuit.output (circuit32 default) 0
 
-example : LawfulCircuit.final_offset (circuit32 default) 0 = 8 := by
-  dsimp only [lawful_norm, lawful, Boolean.circuit]
+example : ExplicitCircuit.final_offset (circuit32 default) 0 = 8 := by
+  dsimp only [explicit_norm, explicit, Boolean.circuit]
 
-example : LawfulCircuit.output (circuit32 default) 0
+example : ExplicitCircuit.output (circuit32 default) 0
     = { z := { x0 := var ⟨0⟩, x1 := var ⟨2⟩, x2 := var ⟨4⟩, x3 := var ⟨6⟩ }, carry_out := var ⟨7⟩ } := by
-  dsimp only [lawful_norm, lawful, Boolean.circuit]
+  dsimp only [explicit_norm, explicit, Boolean.circuit]
 
-open OperationsFrom in
 example (input : Var Inputs (F p)) (env) (i0 : ℕ) :
     Circuit.constraints_hold.soundness env ((circuit32 input).operations i0) := by
   let ⟨ x, y, carry_in ⟩ := input
@@ -27,7 +31,7 @@ example (input : Var Inputs (F p)) (env) (i0 : ℕ) :
   let ⟨ y0, y1, y2, y3 ⟩ := y
 
   -- these are equivalent ways of rewriting the constraints
-  -- the second one relies on prior inference of a `LawfulCircuit` instance
+  -- the second one relies on prior inference of a `ExplicitCircuit` instance
   -- note that the second one only uses a handful of theorems (much fewer than `circuit_norm` + `subcircuit_norm`)
   -- for 90% of the unfolding; and doesn't even need to unfold names like `add32_full` and `add8_full_carry`
 
@@ -37,10 +41,9 @@ example (input : Var Inputs (F p)) (env) (i0 : ℕ) :
   -- dsimp only [circuit_norm, circuit32, add32_full, add8_full_carry, Boolean.circuit]
   -- simp only [subcircuit_norm, circuit_norm]
 
-  -- second version: using `LawfulCircuit`
-  rw [LawfulCircuit.soundness_eq]
-  -- resolve lawful circuit operations
-  dsimp only [lawful_norm, lawful, Boolean.circuit]
+  -- second version: using `ExplicitCircuit`
+  -- resolve explicit circuit operations
+  dsimp only [lawful_norm, explicit, Boolean.circuit]
   -- simp constraints hold expression
   simp only [append_empty, empty_append, append_assoc, append_val, Circuit.constraints_hold.append_soundness, Circuit.constraints_hold.soundness]
   -- simp `eval` and boolean subcircuit soundness
